theories/examples/delim_lang/program_logic/ghost_stacks.v
@@ -1,0 +1,325 @@
+From iris.algebra Require Import auth gmap gset excl frac.
+From iris.base_logic Require Import invariants.
+From iris.proofmode Require Import tactics.
+From iris.bi.lib Require Import fractional.
+
+Definition ghost_id := gname.
+
+Definition gstack := list gname.
+Definition gstackO := listO gnameO.
+
+Definition gsingleton (γ : gname) : gstack := [γ].
+Definition gpush (γ : gname) (s : gstack) : gstack := γ :: s.
+Definition gpop (s : gstack) : gstack := tail s.
+Definition gtop (s : gstack) : option gname := head s.
+
+Lemma gtop_gpush γ s : gtop (gpush γ s) = Some γ.
+Proof. done. Qed.
+Lemma gtop_gsingleton γ : gtop (gsingleton γ) = Some γ.
+Proof. done. Qed.
+Lemma gpop_gpush γ s : gpop (gpush γ s) = s.
+Proof. done. Qed.
+Lemma gtop_inv γ s : gtop s = Some γ → ∃ s', s = gpush γ s'.
+Proof. destruct s; first done; eexists; simplify_eq/=; reflexivity. Qed.
+
+Definition gstackUR := optionUR (exclR gstackO).
+
+Definition gstacks := gmap ghost_id gstack.
+
+Definition gstacksΣ := #[GFunctor (authUR (gsetUR ghost_id)); GFunctor (authUR gstackUR)].
+
+Class gstacksGpre Σ := {
+    gstacksGpre_dom_ing :: inG Σ (authUR (gsetUR ghost_id));
+    gstacksGpre_ing :: inG Σ (authUR gstackUR);
+  }.
+
+Class gstacksIG Σ := {
+    gstacks_dom_ing :: inG Σ (authUR (gsetUR ghost_id));
+    gstacks_ing :: inG Σ (authUR gstackUR);
+    gstacks_name : gname;
+  }.
+
+Global Instance gstacks_subΣ_inG Σ : subG gstacksΣ Σ → gstacksGpre Σ.
+Proof. solve_inG. Qed.
+
+Section ghost_stacks.
+  Context `{!gstacksIG Σ}.
+
+  Definition gstack_frag (n : ghost_id) (s : gstack) : iProp Σ :=
+    own gstacks_name (◯ {[n]}) ∗ own n (◯ Excl' s).
+  Definition gstack_full (n : ghost_id) (s : gstack) : iProp Σ :=
+    own gstacks_name (◯ {[n]}) ∗ own n (● Excl' s).
+
+  Definition gstack_exists (n : ghost_id) : iProp Σ := own gstacks_name (◯ {[n]}).
+
+  Definition gstacks_except (M : gstacks) (N : gset ghost_id) : iProp Σ :=
+    ⌜N ⊆ dom M⌝ ∗ own gstacks_name (● dom M) ∗
+    [∗ map] n ↦ s ∈ M, if bool_decide (n ∈ N) then True else gstack_full n s.
+
+  Global Typeclasses Opaque gstack_frag gstack_full gstacks_except gstack_exists.
+
+  Global Instance gstack_frag_Timeless n s : Timeless (gstack_frag n s).
+  Proof. rewrite /gstack_frag; apply _. Qed.
+  Global Instance gstack_full_Timeless n s : Timeless (gstack_full n s).
+  Proof. rewrite /gstack_full; apply _. Qed.
+  Global Instance gstack_exists_Timeless n : Timeless (gstack_exists n).
+  Proof. rewrite /gstack_exists; apply _. Qed.
+
+  Global Instance gstack_exists_Persistent n : Persistent (gstack_exists n).
+  Proof. rewrite /gstack_exists; apply _. Qed.
+
+  Global Instance gstacks_except_Timeless M N : Timeless (gstacks_except M N).
+  Proof.
+    apply bi.sep_timeless; first apply _.
+    apply bi.sep_timeless; first apply _.
+    apply big_sepM_timeless; intros; destruct bool_decide; apply _.
+  Qed.
+
+  Lemma gstacks_agree n s s' : gstack_full n s -∗ gstack_frag n s' -∗ ⌜s = s'⌝.
+  Proof.
+    rewrite /gstack_frag /gstack_full.
+    iIntros "[_ H1] [_ H2]".
+    iDestruct (own_valid_2 with "H1 H2") as %[Hvl _]%auth_both_valid_discrete; iPureIntro.
+    apply Excl_included, leibniz_equiv in Hvl; done.
+  Qed.
+
+  Lemma gstack_frag_unique n s s' : gstack_frag n s -∗ gstack_frag n s' -∗ False.
+  Proof.
+    rewrite /gstack_frag.
+    iIntros "[_ H1] [_ H2]".
+    iDestruct (own_valid_2 with "H1 H2") as %Hvl.
+    rewrite -auth_frag_op in Hvl.
+    apply auth_frag_valid_1 in Hvl; done.
+  Qed.
+
+  Lemma gstack_full_unique n s s' : gstack_full n s -∗ gstack_full n s' -∗ False.
+  Proof.
+    rewrite /gstack_full.
+    iIntros "[_ H1] [_ H2]".
+    iDestruct (own_valid_2 with "H1 H2") as %Hvl.
+    rewrite auth_auth_op_valid in Hvl; done.
+  Qed.
+
+  Lemma gstack_push n s s' γ :
+    gstack_full n s -∗ gstack_frag n s' ==∗ gstack_full n (gpush γ s) ∗ gstack_frag n (gpush γ s').
+  Proof.
+    iIntros "Hfl Hfr".
+    iDestruct (gstacks_agree with "Hfl Hfr") as %<-.
+    rewrite /gstack_frag /gstack_full.
+    iDestruct "Hfl" as "[$ Hfl]".
+    iDestruct "Hfr" as "[$ Hfr]".
+    iMod (own_update_2 _ _ _ (● _ ⋅ ◯ _) with "Hfl Hfr") as "[$ $]"; last done.
+    apply auth_update, option_local_update, exclusive_local_update; done.
+  Qed.
+
+  Lemma gstack_pop n s s' γ γ' :
+    gstack_full n (gpush γ s) -∗ gstack_frag n (gpush γ' s') ==∗ gstack_full n s ∗ gstack_frag n s'.
+  Proof.
+    iIntros "Hfl Hfr".
+    iDestruct (gstacks_agree with "Hfl Hfr") as %?; simplify_eq.
+    rewrite /gstack_frag /gstack_full.
+    iDestruct "Hfl" as "[$ Hfl]".
+    iDestruct "Hfr" as "[$ Hfr]".
+    iMod (own_update_2 _ _ _ (● _ ⋅ ◯ _) with "Hfl Hfr") as "[$ $]"; last done.
+    apply auth_update, option_local_update, exclusive_local_update; done.
+  Qed.
+
+  Lemma gstack_frag_exists n s : gstack_frag n s -∗ gstack_exists n.
+  Proof. rewrite /gstack_frag /gstack_exists; iIntros "[$ ?]". Qed.
+
+  Lemma gstack_full_exists n s : gstack_full n s -∗ gstack_exists n.
+  Proof. rewrite /gstack_full /gstack_exists; iIntros "[$ ?]". Qed.
+
+  Lemma gstack_exists_in M N n : gstack_exists n -∗ gstacks_except M N -∗ ⌜n ∈ dom M⌝.
+  Proof.
+    rewrite /gstack_exists /gstacks_except.
+    iIntros "H1 (_&H2&_)".
+    iDestruct (own_valid_2 with "H2 H1") as %[?%gset_included ?]%auth_both_valid_discrete.
+    iPureIntro.
+    set_solver.
+  Qed.
+
+  Lemma gstack_frag_in M N n s : gstack_frag n s -∗ gstacks_except M N -∗ ⌜n ∈ dom M⌝.
+  Proof.
+    iIntros "Hfr Hgs".
+    iDestruct (gstack_frag_exists with "Hfr") as "#?".
+    iApply gstack_exists_in; done.
+  Qed.
+
+  Lemma gstack_frag_not_out_agree M N n s :
+    n ∉ N → gstack_frag n s -∗ gstacks_except M N -∗ ⌜M !! n = Some s⌝.
+  Proof.
+    iIntros (?) "Hfr Hgs".
+    iDestruct (gstack_frag_in with "Hfr Hgs") as %[s' Hs']%elem_of_dom.
+    rewrite /gstack_frag /gstacks_except.
+    iDestruct "Hgs" as "[% [? Hfls]]".
+    iDestruct (big_sepM_lookup _ _ n with "Hfls") as "Hfl"; first eassumption.
+    rewrite bool_decide_eq_false_2; last done.
+    iDestruct (gstacks_agree with "Hfl Hfr") as %->; done.
+  Qed.
+
+  Lemma gstack_full_in M N n s : gstack_full n s -∗ gstacks_except M N -∗ ⌜n ∈ dom M⌝.
+  Proof.
+    iIntros "Hfr Hgs".
+    iDestruct (gstack_full_exists with "Hfr") as "#?".
+    iApply gstack_exists_in; done.
+  Qed.
+
+  Lemma gstack_full_is_out M N n s : gstack_full n s -∗ gstacks_except M N -∗ ⌜n ∈ N⌝.
+  Proof.
+    destruct (decide (n ∈ N)); first by auto.
+    iIntros "Hfl Hgs".
+    iDestruct (gstack_full_in with "Hfl Hgs") as %[s' Hs']%elem_of_dom.
+    rewrite /gstacks_except.
+    iDestruct "Hgs" as "[% [? Hfls]]".
+    iDestruct (big_sepM_lookup _ _ n with "Hfls") as "Hfl'"; first eassumption.
+    rewrite bool_decide_eq_false_2; last done.
+    iDestruct (gstack_full_unique with "Hfl Hfl'") as "?"; done.
+  Qed.
+
+  Lemma gstacks_take_out M N n :
+    n ∉ N →
+    gstack_exists n -∗
+    gstacks_except M N -∗ ∃ s, ⌜M !! n = Some s⌝ ∗ gstacks_except M (N ∪ {[n]}) ∗ gstack_full n s.
+  Proof.
+    iIntros (Hn) "#Hex Hgs".
+    iDestruct (gstack_exists_in with "Hex Hgs") as %?.
+    destruct (M !! n) as [s|] eqn:HMn; last first.
+    { apply not_elem_of_dom in HMn; set_solver. }
+    iExists s; iSplit; first done.
+    rewrite /gstacks_except.
+    iDestruct "Hgs" as "(%&$&Hgs)".
+    replace M with (delete n M ∪ {[n := s]}); last first.
+    { apply map_eq; intros i; destruct (decide (i = n)) as [->|].
+      - rewrite lookup_union lookup_singleton lookup_delete //.
+      - rewrite lookup_union lookup_singleton_ne // lookup_delete_ne //.
+        case: (M !! i); done. }
+    assert (delete n M ##ₘ {[n := s]}).
+    { apply map_disjoint_spec; intros i ? ? Hdl [-> ->]%lookup_singleton_Some.
+      rewrite lookup_delete in Hdl; done. }
+    repeat (rewrite big_sepM_union; last done).
+    rewrite !big_sepM_singleton.
+    rewrite bool_decide_eq_false_2; last set_solver.
+    rewrite bool_decide_eq_true_2; last set_solver.
+    iDestruct "Hgs" as "[Hgs $]".
+    iSplit; first by iPureIntro; set_solver.
+    iSplit; last done.
+    iApply big_sepM_mono; last iAssumption.
+    intros i ? ?; simpl.
+    destruct (decide (i = n)) as [->|].
+    { rewrite [bool_decide (n ∈ N ∪ _)]bool_decide_eq_true_2; [auto|set_solver]. }
+    destruct (decide (i ∈ N)).
+    { repeat (rewrite bool_decide_eq_true_2; last set_solver); done. }
+    { repeat (rewrite bool_decide_eq_false_2; last set_solver); done. }
+  Qed.
+
+  Lemma gstacks_put_back M N n s :
+    M !! n = Some s →
+    gstack_full n s -∗ gstacks_except M N -∗ gstacks_except M (N ∖ {[n]}).
+  Proof.
+    iIntros (HMns) "Hfl Hgs".
+    iDestruct (gstack_full_is_out with "Hfl Hgs") as %?.
+    rewrite /gstacks_except.
+    iDestruct "Hgs" as "[% [$ Hgs]]".
+    iSplit; first by iPureIntro; set_solver.
+    replace M with (delete n M ∪ {[n := s]}); last first.
+    { apply map_eq; intros i; destruct (decide (i = n)) as [->|].
+      - rewrite lookup_union lookup_singleton lookup_delete //.
+      - rewrite lookup_union lookup_singleton_ne // lookup_delete_ne //.
+        case: (M !! i); done. }
+    assert (delete n M ##ₘ {[n := s]}).
+    { apply map_disjoint_spec; intros i ? ? Hdl [-> ->]%lookup_singleton_Some.
+      rewrite lookup_delete in Hdl; done. }
+    repeat (rewrite big_sepM_union; last done).
+    iDestruct "Hgs" as "[Hgs _]".
+    rewrite !big_sepM_singleton.
+    rewrite bool_decide_eq_false_2; last set_solver.
+    iFrame "Hfl".
+    iApply big_sepM_mono; last iAssumption.
+    intros i ? Hnmi; simpl.
+    assert (i ≠ n).
+    { intros ->; rewrite lookup_delete in Hnmi; done. }
+    destruct (decide (i ∈ N)).
+    { repeat (rewrite bool_decide_eq_true_2; last set_solver); done. }
+    { repeat (rewrite bool_decide_eq_false_2; last set_solver); done. }
+  Qed.
+
+  Lemma gstacks_out_swap M N n s :
+    n ∈ N → gstacks_except M N -∗ gstacks_except (<[n := s]>M) N.
+  Proof.
+    rewrite /gstacks_except.
+    iIntros (HnN) "HM".
+    iDestruct "HM" as "[% HM]".
+    assert (dom (<[n := s]> M) = dom M) as Hdomeq by set_solver.
+    rewrite Hdomeq.
+    iSplit; first done.
+    iDestruct "HM" as "[$ HM]".
+    destruct (M !! n) as [s'|] eqn:Heq; last first.
+    { apply not_elem_of_dom in Heq; set_solver. }
+    replace M with (delete n M ∪ {[n := s']}); last first.
+    { apply map_eq; intros i; destruct (decide (i = n)) as [->|].
+      - rewrite lookup_union lookup_singleton lookup_delete //.
+      - rewrite lookup_union lookup_singleton_ne // lookup_delete_ne //.
+        case: (M !! i); done. }
+    assert (delete n M ##ₘ {[n := s']}).
+    { apply map_disjoint_spec; intros i ? ? Hdl [-> ->]%lookup_singleton_Some.
+      rewrite lookup_delete in Hdl; done. }
+    replace (<[n:=s]> (delete n M ∪ {[n := s']})) with (delete n M ∪ {[n := s]}); last first.
+    { apply map_eq; intros i. destruct (decide (i = n)) as [->|].
+      - rewrite lookup_insert lookup_union lookup_delete lookup_singleton //.
+      - rewrite lookup_insert_ne // !lookup_union !lookup_singleton_ne //. }
+    assert (delete n M ##ₘ {[n := s]}).
+    { apply map_disjoint_spec; intros i ? ? Hdl [-> ->]%lookup_singleton_Some.
+      rewrite lookup_delete in Hdl; done. }
+    repeat (rewrite big_sepM_union; last done).
+    iDestruct "HM" as "[HM _]".
+    rewrite !big_sepM_singleton.
+    rewrite bool_decide_eq_true_2; last done.
+    iSplit; last done.
+    iApply big_sepM_mono; last iAssumption.
+    intros i ? Hnmi; simpl.
+    assert (i ≠ n).
+    { intros ->; rewrite lookup_delete in Hnmi; done. }
+    destruct (decide (i ∈ N)).
+    { repeat (rewrite bool_decide_eq_true_2; last set_solver); done. }
+    { repeat (rewrite bool_decide_eq_false_2; last set_solver); done. }
+  Qed.
+
+  Lemma gstacks_except_included M N : gstacks_except M N -∗ ⌜N ⊆ dom M⌝.
+  Proof. rewrite /gstacks_except; iIntros "[% ?]"; done. Qed.
+
+  Lemma gstack_alloc M N :
+    gstacks_except M N ==∗ ∃ n, ⌜n ∉ dom M⌝ ∗ gstacks_except (<[n := []]>M) N ∗ gstack_frag n [].
+  Proof.
+    rewrite /gstacks_except /gstack_full /gstack_frag.
+    iIntros "(%&Hdm&HM)".
+    iMod (own_alloc_cofinite (● Excl' [] ⋅ ◯ Excl' []) (dom M)) as (n) "[%HnM [Hfl Hfr]]".
+    { apply auth_both_valid_2; done. }
+    iMod (own_update _ _ (● ({[n]} ∪ dom M) ⋅ ◯ ({[n]} ∪ dom M)) with "Hdm") as "[Hdm Hn]".
+    { apply auth_update_alloc; apply gset_local_update; set_solver. }
+    iAssert (own gstacks_name (◯ {[n]})) as "#?".
+    { rewrite -gset_op; iDestruct "Hn" as "[$ _]". }
+    iModIntro.
+    iExists n.
+    iSplit; first done.
+    iFrame "#".
+    rewrite dom_insert.
+    iFrame "Hfr Hdm".
+    iSplit; first by iPureIntro; set_solver.
+    rewrite big_sepM_insert; last by apply not_elem_of_dom.
+    rewrite bool_decide_eq_false_2; last set_solver.
+    iFrame "#"; iFrame.
+  Qed.
+
+End ghost_stacks.
+
+Lemma gstacks_init `{!gstacksGpre Σ} : ⊢ |==> ∃ _ : gstacksIG Σ, gstacks_except ∅ ∅.
+Proof.
+  rewrite /gstacks_except.
+  iIntros "".
+  iMod (own_alloc (● ∅)) as (γ) "Hdm"; first by apply auth_auth_valid.
+  iModIntro.
+  iExists {| gstacks_name := γ |}.
+  iSplit; first done.
+  rewrite dom_empty big_sepM_empty; auto.
+Qed.
