theories/examples/delim_lang/program_logic/lib/sts.v
@@ -1,0 +1,221 @@
+From iris.algebra Require Import auth gmap.
+From iris.base_logic Require Import invariants.
+From iris.algebra Require Import mra.
+From iris.proofmode Require Import proofmode.
+From WBLogic.program_logic Require Import ghost_stacks weakestpre.
+
+Record STS := {
+  STS_state :> Type;
+  state_inh :: Inhabited STS_state;
+  pub_rel : STS_state → STS_state → Prop;
+  pri_rel : STS_state → STS_state → Prop;
+  pub_rel_po :: PreOrder pub_rel;
+  pri_rel_po :: PreOrder pri_rel;
+  pub_pri_incl : ∀ s s', pub_rel s s' → pri_rel s s'
+}.
+
+Definition STSUR (S : STS) := authUR (mraUR (pub_rel S)).
+
+Definition STSΣ S : gFunctors := #[GFunctor (STSUR S)].
+
+Global Instance subG_STSΣ_ing S Σ : subG (STSΣ S) Σ → inG Σ (STSUR S).
+Proof. solve_inG. Qed.
+
+Section STS.
+  Context {S} `{!irisGS Λ Σ, !inG Σ (STSUR S), !gstacksIG Σ}.
+
+  Definition sts_config : Type := gstack * S.
+
+  Definition state_of (sc : sts_config) : S := sc.2.
+
+  Definition related_public (sc sc' : sts_config) : iProp Σ :=
+    ⌜sc.1 = sc'.1⌝ ∗ ⌜pub_rel S (state_of sc) (state_of sc')⌝.
+
+  Definition related_private (sc sc' : sts_config) : iProp Σ :=
+    ∃ γ γ', ⌜sc'.1 = gpush γ' sc.1⌝ ∗ ⌜gtop sc.1 = Some γ⌝ ∗
+      own γ (● (to_mra (state_of sc))) ∗ ⌜pri_rel S (state_of sc) (state_of sc')⌝.
+
+  Definition STS_inv_name (N : ghost_id) := nroot.@"gstack".@N.
+
+  Definition sts_config_frag N (sc : sts_config) : iProp Σ :=
+    ∃ γ, gstack_full N sc.1 ∗ ⌜gtop sc.1 = Some γ⌝ ∗ own γ (◯ (to_mra sc.2)).
+
+  Definition sts_config_full N (sc : sts_config) : iProp Σ :=
+    (∃ γ, gstack_frag N sc.1 ∗ ⌜gtop sc.1 = Some γ⌝ ∗ own γ (● (to_mra sc.2))).
+
+  Definition STS_inv (N : ghost_id) (P : S → iProp Σ) : iProp Σ :=
+    inv (STS_inv_name N) (∃ sc, sts_config_full N sc ∗ P (state_of sc)).
+
+  Lemma sts_configs_update_frag N sc sc' :
+    sts_config_full N sc ⊢ sts_config_frag N sc' ==∗ sts_config_full N sc ∗ sts_config_frag N sc.
+  Proof.
+    iDestruct 1 as (?) "(Hstfr & % & Hprfl)".
+    iDestruct 1 as (?) "(Hstfl & % & Hprfr)".
+    iDestruct (gstacks_agree with "Hstfl Hstfr") as %?.
+    destruct sc; destruct sc'; simplify_eq/=.
+    iDestruct (own_valid_2 with "Hprfl Hprfr") as %[Hincl ?]%auth_both_valid_discrete.
+    rewrite to_mra_included in Hincl.
+    iClear "Hprfr".
+    iMod (own_update with "Hprfl") as "[Hprfl Hprfr]".
+    { apply auth_update_alloc; apply mra_local_update_grow; reflexivity. }
+    iModIntro.
+    iSplitL "Hstfr Hprfl"; iFrame; iExists _; iFrame; done.
+  Qed.
+
+  Lemma sts_configs_pub_related N sc sc' :
+    sts_config_full N sc ⊢ sts_config_frag N sc' -∗ related_public sc' sc.
+  Proof.
+    iDestruct 1 as (?) "(Hstfr & % & Hprfl)".
+    iDestruct 1 as (?) "(Hstfl & % & Hprfr)".
+    iDestruct (gstacks_agree with "Hstfl Hstfr") as %?.
+    destruct sc; destruct sc'; simplify_eq/=.
+    iDestruct (own_valid_2 with "Hprfl Hprfr") as %[Hincl ?]%auth_both_valid_discrete.
+    rewrite to_mra_included in Hincl; done.
+  Qed.
+
+  Lemma related_private_public sc sc' sc'' :
+    related_private sc sc' ⊢ related_public sc' sc'' -∗ related_private sc sc''.
+  Proof.
+    destruct sc as [? ?]; destruct sc' as [? ?]; destruct sc'' as [? ?].
+    iDestruct 1 as (? ?) "(%&%& HPrfl &%)".
+    iIntros "[% %]".
+    simplify_eq/=.
+    iExists _, _; iFrame; simpl.
+    iSplit; first done.
+    iSplit; first done.
+    iPureIntro.
+    etrans; first eassumption.
+    by apply pub_pri_incl.
+  Qed.
+
+  Lemma related_public_trans sc sc' sc'' :
+    related_public sc sc' ⊢ related_public sc' sc'' -∗ related_public sc sc''.
+  Proof.
+    destruct sc as [? ?]; destruct sc' as [? ?]; destruct sc'' as [? ?].
+    iIntros "[% %] [% %]"; simplify_eq/=; iSplit; iPureIntro; first done.
+    etrans; eassumption.
+  Qed.
+
+  Lemma related_public_states sc sc' :
+    related_public sc sc' ⊢ ⌜pub_rel S (state_of sc) (state_of sc')⌝.
+  Proof. iIntros "[% %]"; done. Qed.
+
+  Lemma sts_make_public_trans N sc s' :
+    pub_rel S (state_of sc) s' →
+    sts_config_frag N sc ⊢ sts_config_full N sc ==∗
+      ∃ sc', related_public sc sc' ∗ ⌜state_of sc' = s'⌝ ∗ sts_config_frag N sc' ∗ sts_config_full N sc'.
+  Proof.
+    destruct sc as [? s].
+    iIntros (?).
+    iDestruct 1 as (γ) "(Hfl & % & _)".
+    iDestruct 1 as (γ') "(Hfr & % & HPrfl)".
+    simplify_eq/=.
+    iMod (own_update with "HPrfl") as "[HPrfl HPrfr]".
+    { apply auth_update_alloc; apply mra_local_update_grow; eassumption. }
+    iModIntro; iExists (_, s').
+    iSplit; first done. iSplit; first done.
+    iSplitL "Hfl HPrfr"; iExists _; iFrame; done.
+  Qed.
+
+  Lemma sts_make_private_trans N sc s' :
+    pri_rel S (state_of sc) s' →
+    sts_config_frag N sc ⊢ sts_config_full N sc ==∗
+      ∃ sc', related_private sc sc' ∗ ⌜state_of sc' = s'⌝ ∗ sts_config_frag N sc' ∗ sts_config_full N sc'.
+  Proof.
+    destruct sc as [? s].
+    iIntros (?).
+    iDestruct 1 as (γ) "(Hfl & Htop & _)".
+    iDestruct "Htop" as %[? ?]%gtop_inv.
+    iDestruct 1 as (γ') "(Hfr & % & HPrfl)".
+    simplify_eq/=.
+    iMod (own_alloc (● (to_mra s') ⋅ ◯ (to_mra s'))) as (γ'') "[HPrfl' HPrfr]";
+      first by apply auth_both_valid.
+    iMod (gstack_push _ _ _ γ'' with "Hfl Hfr") as "[Hfl Hfr]".
+    iModIntro; iExists (_, s').
+    iSplitL "HPrfl".
+    { iExists _, _; iFrame; eauto. }
+    iSplit; first done.
+    iSplitL "Hfl HPrfr"; iExists _; iFrame; done.
+  Qed.
+
+  Lemma sts_make_undo_private_trans N sc sc' :
+    related_private sc sc' ⊢
+    sts_config_frag N sc' -∗ sts_config_full N sc' ==∗ sts_config_frag N sc ∗ sts_config_full N sc.
+  Proof.
+    destruct sc as [? s]; destruct sc' as [? s'].
+    iDestruct 1 as (? ?) "(% & % & HPrfl & %)".
+    simplify_eq/=.
+    iDestruct 1 as (γ1) "(Hfl & Htop & _)".
+    iDestruct "Htop" as %[? ?]%gtop_inv.
+    iDestruct 1 as (γ2) "(Hfr & % & _)".
+    simplify_eq/=.
+    iMod (gstack_pop with "Hfl Hfr") as "[Hfl Hfr]".
+    iMod (own_update with "HPrfl") as "[HPrfl HPrfr]".
+    { apply auth_update_alloc; apply mra_local_update_grow; reflexivity. }
+    iModIntro.
+    iSplitL "HPrfr Hfl".
+    { iExists _; iFrame; eauto. }
+    iExists _; iFrame; done.
+  Qed.
+
+  Lemma make_STS {E N} (s : S) (P : S → iProp Σ) :
+    P s ⊢ gstack_full N [] -∗ gstack_frag N [] -∗ |={E}=> STS_inv N P ∗ ∃ stk, gstack_full N stk.
+  Proof.
+    iIntros "HP Hfl Hfr".
+    iMod (own_alloc (● (to_mra s))) as (γ) "Hs"; first by apply auth_auth_valid.
+    iMod (gstack_push _ _ _ γ with "Hfl Hfr") as "[Hfl Hfr]".
+    iMod (inv_alloc (STS_inv_name N) _
+      (∃ sc, sts_config_full N sc ∗ P sc.2)%I with "[- Hfl]")
+    as "#Hinv".
+    { iNext. iExists (_, _); iFrame "HP Hfr". iExists _; iFrame; done. }
+    iModIntro; iFrame "#".
+    iExists _; iFrame.
+  Qed.
+
+  Lemma wbwp_sts_get_state E N P out e Φ :
+    ↑(STS_inv_name N) ⊆ E →
+    N ∉ out →
+    STS_inv N P -∗
+    (∀ sc, sts_config_frag N sc -∗
+      WBWP e @ (out ∪ {[N]}); E {{v, Φ v ∗ ∃ sc', sts_config_frag N sc' ∗ related_public sc sc' }}) -∗
+    WBWP e @ out; E {{ Φ }}.
+  Proof.
+    iIntros (? ?) "#Hinv HWBWP".
+    iAssert (|={E}=> gstack_exists N)%I as ">#Hex".
+    { iInv (STS_inv_name N) as (?) "[>Hfl ?]". iDestruct "Hfl" as (?) "(? & ?)".
+      iDestruct (gstack_frag_exists with "[$]") as "#?".
+      iModIntro. iSplitL; last done. iNext. iExists _; iFrame. iExists _; iFrame. }
+    iApply (wbwp_get_gstack_full with "[$] [HWBWP]"); first done.
+    iIntros (stk) "Hfl".
+    iApply fupd_wbwp.
+    iInv (STS_inv_name N) as (?) "(>Hscfl & Hrest)" "Hcl".
+    iDestruct "Hscfl" as (?) "(Hfr & % & Hstsfl)".
+    iDestruct (gstacks_agree with "Hfl Hfr") as %?; subst.
+    iMod (own_update with "Hstsfl") as "[Hstsfl Hstsfr]".
+    { apply auth_update_alloc; apply mra_local_update_grow; reflexivity. }
+    iMod ("Hcl" with "[Hfr Hrest Hstsfl]") as "_".
+    { iNext; iExists _; iFrame; iExists _; iFrame; done. }
+    iModIntro.
+    iApply (wbwp_wand with "[-]").
+    { iApply ("HWBWP" $! (_, _)). iExists _; iFrame; done. }
+    simpl.
+    iIntros (w) "[$ Hsc']".
+    iDestruct "Hsc'" as ([]) "[Hsc' [% %]]"; simplify_eq/=.
+    iDestruct "Hsc'" as (?) "[$ ?]".
+  Qed.
+
+  Lemma wbwp_sts_mend N sc E out e Φ :
+    sts_config_frag N sc -∗
+    WBWP e @ out ∖ {[N]}; E {{ Φ }} -∗
+    WBWP e @ out; E {{v, sts_config_frag N sc ∗ Φ v }}.
+  Proof.
+    iIntros "Hfl HWBWP".
+    iDestruct "Hfl" as (γ) "(Hfl&%&?)".
+    iApply (wbwp_wand with "[Hfl HWBWP]").
+    { iApply (wbwp_mend with "Hfl HWBWP"). }
+    iIntros (v) "[? $]"; iExists _; iFrame; done.
+  Qed.
+
+End STS.
+
+Global Arguments sts_config _ : clear implicits.
