theories/examples/delim_lang/program_logic/lifting.v
@@ -1,0 +1,59 @@
+(** This file has been taken from iris and edited accordingly. *)
+(** The "lifting lemmas" in this file serve to lift the rules of the operational
+semantics to the program logic. *)
+
+From iris.proofmode Require Import proofmode.
+From iris.program_logic Require Import lifting.
+From gitrees Require Export examples.delim_lang.program_logic.weakestpre.
+From iris.prelude Require Import options.
+
+Section lifting.
+  Context {n : nat} {a : is_ctx_dep} (rs : gReifiers a n) {A} `{!Cofe A}.
+  Notation rG := (gReifiers_sReifier rs).
+  Notation F := (sReifier_ops rG).
+  Notation IT := (IT F A).
+  Notation ITV := (ITV F A).
+  Notation stateF := (gReifiers_state rs).
+  Notation stateO := (stateF ♯ IT).
+  Notation stateR := (gReifiers_ucmra rs IT).
+  Let of_state := (of_state rs IT).
+  Let of_idx := (of_idx rs IT).
+  Notation reify := (reify rG).
+  Notation istep := (istep rG).
+  Notation isteps := (isteps rG).
+  Notation sstep := (sstep rG).
+  Notation ssteps := (ssteps rG).
+
+  Implicit Type op : opid F.
+  Implicit Type α β : IT.
+
+  Context `{!invGS Σ} `{!stateG rs A Σ} `{!gstacksIG Σ}.
+  Notation iProp := (iProp Σ).
+  Notation coPsetO := (leibnizO coPset).
+
+  (* Lemma wbwp_pure_step_fupd E E' out e1 e2 φ m Φ : *)
+  (*   (* PureExec φ n e1 e2 → *) *)
+  (*   φ → *)
+  (*   (|={E}[E']▷=>^n £ m *)
+  (*    -∗ WBWP@{rs} e2 @ out; E {{ Φ }}) ⊢ WBWP@{rs} e1 @ out; E {{ Φ }}. *)
+  (* Proof. *)
+  (*   rewrite /wbwp. *)
+  (*   iIntros ((* Hexec *) Hφ) "Hwp". *)
+  (*   iIntros (M) "HM". *)
+  (*   iApply wp_pure_step_fupd; first done. *)
+  (*   iApply (step_fupdN_wand with "Hwp"). *)
+  (*   iIntros "Hwp H". *)
+  (*   iSpecialize ("Hwp" with "H HM"); done. *)
+  (* Qed. *)
+
+  (* Lemma wbwp_pure_step_later `{!Inhabited (state Λ)} E out e1 e2 φ n Φ : *)
+  (*   PureExec φ n e1 e2 → *)
+  (*   φ → *)
+  (*   ▷^n (£ n -∗ WBWP e2 @ out; E {{ Φ }}) ⊢ WBWP e1 @ out; E {{ Φ }}. *)
+  (* Proof. *)
+  (*   intros Hexec ?. rewrite -wbwp_pure_step_fupd //. clear Hexec. *)
+  (*   enough (∀ P, ▷^n P -∗ |={E}▷=>^n P) as Hwp by iApply Hwp. iIntros (?). *)
+  (*   induction n as [|n IH]; simpl; first by auto. *)
+  (*   iIntros; rewrite -step_fupd_intro; last done. iNext; iApply IH; done. *)
+  (* Qed. *)
+End lifting.
